proof/SimProg.v
@@ -33,7 +33,7 @@ Context `{SM: SimMem.class} {SS: SimSymb.class SM} {SU: Sound.class}.
   Definition simU_aux {SMOS: SimMemOhs.class} (pp: t) (begin: Midx.t) :=
     let ppi := Midx.mapi_aux (fun i x => (i, x)) begin pp in
     List.Forall (fun '(i, x) => ModPair.simU x i) ppi.
-  Definition simU {SMOS: SimMemOhs.class} (pp: t) := simU_aux pp 0%nat.
+  Definition simU {SMOS: SimMemOhs.class} (pp: t) := simU_aux pp 1%nat.
 
   Definition src (pp: t): program := List.map ModPair.src pp.
   Definition tgt (pp: t): program := List.map ModPair.tgt pp.
@@ -102,8 +102,102 @@ Context `{SM: SimMem.class} {SS: SimSymb.class SM} {SU: Sound.class}.
 
 End SIM.
 
+Module WEMANYNOTNEETHIS.
+Section SIM.
+Context `{SM: SimMem.class} {SS: SimSymb.class SM}.
+
+  Variable pp: ProgPair.t.
+  Hypothesis SIMPROG:
+    Forall (fun mp =>
+              (<<SIMSK: SimSymb.wf mp.(ModPair.ss)>>) /\
+              (<<SKSRC: mp.(ModPair.ss).(SimSymb.src) = (Mod.sk mp.(ModPair.src))>>) /\
+              (<<SKTGT: mp.(ModPair.ss).(SimSymb.tgt) = (Mod.sk mp.(ModPair.tgt))>>)) pp
+  .
+  Let p_src := (ProgPair.src pp).
+  Let p_tgt := (ProgPair.tgt pp).
 
 
+  Theorem sim_link_sk_aux_aux
+          sk_link_src
+          (LOADSRC: (link_sk p_src) = Some sk_link_src)
+          (WF: forall md, In md p_src -> <<WF: Sk.wf md>>):
+      exists ss_link sk_link_tgt,
+        <<LOADTGT: (link_sk p_tgt) = Some sk_link_tgt>>
+        /\ <<SIMSK: SimSymb.wf ss_link>>
+        /\ <<SKSRC: ss_link.(SimSymb.src) = sk_link_src>>
+        /\ <<SKTGT: ss_link.(SimSymb.tgt) = sk_link_tgt>>
+        /\ <<LE: Forall (fun mp => (SimSymb.le mp.(ModPair.ss) ss_link)) pp>>.
+  Proof.
+    u. subst_locals. ginduction pp; ii; ss. destruct a; ss.
+    unfold ProgPair.src in *. unfold link_sk in *. ss. destruct (classic (t = [])).
+    { clarify; ss. cbn in *. clarify. clear IHt. inv SIMPROG. ss. inv H2. des.
+      esplits; eauto. econs; eauto. ss. refl.
+    }
+    rename H into NNIL. eapply link_list_cons_inv in LOADSRC; cycle 1.
+    { destruct t; ss. }
+    des. rename sk_link_src into sk_link_link_src. rename restl into sk_link_src.
+    inv SIMPROG. exploit IHt; eauto. intro IH; des.
+    clarify. ss. exploit (SimSymb.wf_link).
+    3: { rewrite SKSRC. eapply HD. }
+    all: eauto.
+    { rewrite SKSRC. eapply WF; et. }
+    { eapply link_list_preserves_wf_sk; eauto. }
+    { eapply SimSymb.wf_preserves_wf; et. rewrite SKSRC. eapply WF; et. }
+    { eapply SimSymb.wf_preserves_wf; et. eapply link_list_preserves_wf_sk; eauto. }
+    i; des. esplits; eauto.
+    - eapply link_list_cons; eauto.
+      rewrite SKTGT in LINKTGT. ss.
+    - econs; eauto. rewrite Forall_forall in *. ii.
+      all ltac:(fun H => apply link_list_linkorder in H). des.
+      rewrite Forall_forall in *. etrans; eauto.
+  Qed.
+
+End SIM.
+
+
+Section SIM.
+Context `{SM: SimMem.class} {SMOS: SimMemOhs.class} {SS: SimSymb.class SM} {SU: Sound.class}.
+
+  Variable pp: ProgPair.t.
+  Let p_src := (ProgPair.src pp).
+  Let p_tgt := (ProgPair.tgt pp).
+
+  Theorem sim_link_sk_aux
+          j
+          (SIMPROG: ProgPair.simU_aux pp j)
+          sk_link_src
+          (LOADSRC: (link_sk p_src) = Some sk_link_src)
+          (WF: forall md, In md p_src -> <<WF: Sk.wf md>>):
+      exists ss_link sk_link_tgt,
+        <<LOADTGT: (link_sk p_tgt) = Some sk_link_tgt>>
+        /\ <<SIMSK: SimSymb.wf ss_link>>
+        /\ <<SKSRC: ss_link.(SimSymb.src) = sk_link_src>>
+        /\ <<SKTGT: ss_link.(SimSymb.tgt) = sk_link_tgt>>
+        /\ <<LE: Forall (fun mp => (SimSymb.le mp.(ModPair.ss) ss_link)) pp>>.
+  Proof.
+    eapply sim_link_sk_aux_aux; eauto. rr in SIMPROG. clear - SIMPROG.
+    ginduction pp; ii; ss.
+    inv SIMPROG. econs; eauto.
+    { inv H1. ss. }
+  Qed.
+
+  Theorem sim_link_sk
+          (SIMPROG: ProgPair.simU pp)
+          sk_link_src
+          (LOADSRC: (link_sk p_src) = Some sk_link_src)
+          (WF: forall md, In md p_src -> <<WF: Sk.wf md>>):
+      exists ss_link sk_link_tgt,
+        <<LOADTGT: (link_sk p_tgt) = Some sk_link_tgt>>
+        /\ <<SIMSK: SimSymb.wf ss_link>>
+        /\ <<SKSRC: ss_link.(SimSymb.src) = sk_link_src>>
+        /\ <<SKTGT: ss_link.(SimSymb.tgt) = sk_link_tgt>>
+        /\ <<LE: Forall (fun mp => (SimSymb.le mp.(ModPair.ss) ss_link)) pp>>.
+  Proof.
+    eapply sim_link_sk_aux; eauto.
+  Qed.
+
+End SIM.
+End WEMANYNOTNEETHIS.
 
 
 
@@ -150,15 +244,14 @@ Proof.
         ).
   { admit "cons theorem". }
   clear - H.
-  des.
-  exists SMOS'. rr. rewrite Forall_forall. intros [i x] IN.
-  rewrite Midx.in_mapi_aux_iff in IN. des. clarify. destruct i; ss; clarify.
-  rr in SIM. rewrite Forall_forall in SIM.
-  exploit SIM; eauto.
-  { eapply Midx.in_mapi_aux_iff. esplits; eauto. }
-  i; des. des_ifs.
-  econs; eauto.
-  -
-  econs; eauto.
+  admit "".
+  (* des. *)
+  (* exists SMOS'. rr. rewrite Forall_forall. intros [i x] IN. *)
+  (* rewrite Midx.in_mapi_aux_iff in IN. des. clarify. destruct idx; ss; clarify. *)
+  (* rr in SIM. rewrite Forall_forall in SIM. *)
+  (* exploit SIM; eauto. *)
+  (* { eapply Midx.in_mapi_aux_iff. esplits; eauto. } *)
+  (* i; des. des_ifs. *)
+  (* admit "TODO----------------------------------". *)
 Qed.
-SimModSemUnified.fundamental_theorem
+(* SimModSemUnified.fundamental_theorem *)
