lib/Any.v
@@ -1,0 +1,83 @@
+Require Import sflib CoqlibC.
+Require Import Program.
+Require Import ClassicalDescription EquivDec.
+
+Set Implicit Arguments.
+
+Notation Any := { ty: Type & ty }.
+(* Definition Any := { ty: Type & ty }. *)
+(* Hint Unfold Any. *)
+
+Definition downcast {T: Type} (a: Any): option T.
+  destruct a.
+  destruct (excluded_middle_informative (x = T)).
+  - subst. apply Some. assumption.
+  - apply None.
+Defined.
+
+Definition upcast {T} (a: T): Any := existT (fun x => x) _ a.
+Hint Unfold downcast upcast.
+
+Lemma downcast_spec
+      a T (t: T)
+      (CAST: downcast a = Some t)
+  :
+    <<TY: projT1 a = T>> /\ <<VAL: projT2 a ~= t>>
+.
+Proof.
+  unfold downcast in *. des_ifs. ss.
+  simpl_depind. eauto.
+Qed.
+
+Lemma downcast_intro
+      a T (t: T)
+      (TY: projT1 a = T)
+      (VAL: projT2 a ~= t)
+  :
+    <<CAST: downcast a = Some t>>
+.
+Proof.
+  unfold downcast in *. des_ifs. ss.
+  dependent destruction e. ss.
+Qed.
+
+Lemma upcast_downcast
+      T (a: T)
+  :
+    downcast (upcast a) = Some a
+.
+Proof.
+  eapply downcast_intro; ss.
+Qed.
+
+Lemma upcast_intro
+      (a: Any)
+  :
+    <<CAST: a = upcast (projT2 a)>>
+.
+Proof.
+  unfold upcast in *. dependent destruction a. ss.
+Qed.
+
+Lemma upcast_downcast_iff
+      (a: Any) T (t: T)
+  :
+    <<UPCAST: a = upcast t>> <-> <<DOWNCAST: downcast a = Some t>>
+.
+Proof.
+  split; ii; des.
+  - clarify. rewrite upcast_downcast. ss.
+  - apply downcast_spec in H. des. r.
+    rewrite upcast_intro with a. unfold upcast. simpl_depind. f_equal. ss.
+Qed.
+
+Definition Any_dec (a0 a1: Any): {a0=a1} + {a0<>a1}.
+  destruct a0, a1.
+  simpl_depind.
+  destruct (excluded_middle_informative (x = x0)).
+  - clarify.
+    destruct (excluded_middle_informative (p = p0)).
+    + clarify. left. rewrite sigT_eta. ss.
+    + right. ii. simpl_depind. clarify.
+  - right. ii. simpl_depind.
+Defined.
