proof/SemPreservation.v
@@ -1,0 +1,186 @@
+Require Import CoqlibC.
+Require Import LinkingC.
+Require Import Skeleton.
+Require Import Values.
+Require Import JMeq.
+Require Import Smallstep.
+Require Import Simulation.
+Require Import Integers.
+Require Import EventsC.
+Require Import MapsC.
+Require Import BehaviorsC.
+
+Require Import ModSem Mod Sem.
+
+Require Import Any.
+
+Set Implicit Arguments.
+
+
+
+Module SemPrsv.
+Section PRSV.
+
+  Local Open Scope pair_scope.
+
+  Theorem sound_genv: forall
+      p sk_link mss
+      (LINK: link_sk p = Some sk_link)
+      (MSS: (Sem.sem p).(Smallstep.globalenv)#1 = mss)
+    ,
+      (<<NTHIDX: forall
+          n ms
+          (NTH: nth_error mss n = Some ms)
+        ,
+          (<<IDX: ms.(ModSem.midx) = n>>)>>)
+      /\
+      (<<IDXNTH: forall
+          n ms
+          (IN: In ms mss)
+          (IDX: ms.(ModSem.midx) = n)
+        ,
+          (<<NTH: nth_error mss n = Some ms>>)>>)
+      /\
+      (<<UNIQ: forall
+          ms0 ms1
+          (IN0: In ms0 mss)
+          (IN1: In ms1 mss)
+          (IDX: ms0.(ModSem.midx) = ms1.(ModSem.midx))
+        ,
+          ms0 = ms1>>)
+      (* /\ *)
+      (* (<<FIND: forall *)
+      (*     n ms *)
+      (*     (FIND: find (fun ms => (ms.(ModSem.midx) =? n)%nat) mss = Some ms) *)
+      (*   , *)
+      (*     (<<NTH: nth_error mss n = Some ms>>)>>) *)
+  .
+  Proof.
+    ii. dsplits.
+    -
+      ii. des. subst mss. ss. des_ifs.
+      destruct n; ss; clarify.
+      clear - NTH.
+      unfold load_modsems in *.
+      rewrite Midx.nth_error_mapi_iff in *. des. clarify.
+      eapply Mod.get_modsem_midx_spec; ss.
+    -
+      ii. des. subst mss. ss. des_ifs.
+      unfold load_genv, load_modsems in *. ss.
+      destruct (ModSem.midx ms) eqn:T; ss.
+      { des; ss; clarify. rewrite Midx.in_mapi_iff in IN. des; ss. clarify.
+        unfold Mod.modsem in *. rewrite Mod.get_modsem_midx_spec in T. xomega. }
+      des; ss; clarify.
+      rewrite Midx.in_mapi_iff in IN. des; ss. clarify.
+      unfold Mod.modsem in *. rewrite Mod.get_modsem_midx_spec in T. clarify.
+      eapply Midx.nth_error_mapi_iff. esplits; eauto.
+    -
+      ii. des. subst mss. ss. des_ifs.
+      exploit SPLITHINT0; try apply IN0; eauto. intro T0.
+      exploit SPLITHINT0; try apply IN1; eauto. intro T1.
+      des; clarify.
+  Qed.
+
+  Variable p: program.
+
+  (* Variable sk_link: Sk.t. *)
+  (* Hypothesis LINK: (link_sk p) = Some sk_link. *)
+  (* Let skenv_link := (Sk.load_skenv sk_link). *)
+  Let sem := Sem.sem p.
+
+  Definition frames (st: state): list Frame.t :=
+    match st with
+    | Callstate _ frs _ => frs
+    | State frs _ => frs
+    end
+  .
+
+  Definition sound_state (st: state): Prop :=
+    (<<WTY: forall
+        n ms
+        (NTH: nth_error (sem.(globalenv) #1) n = Some ms)
+      ,
+        (<<TY: projT1 ((get_ohs st) n) = ms.(ModSem.owned_heap)>>)>>)
+    /\
+    (<<LINK: exists sk_link, link_sk p = Some sk_link>>)
+    /\
+    (<<FRAMES: Forall (fun fr => In fr.(Frame.ms) (sem.(globalenv) #1)) (frames st)>>)
+  .
+
+  Theorem sound_initial
+          st
+          (INIT: sem.(Smallstep.initial_state) st)
+    :
+      <<SS: sound_state st>>
+  .
+  Proof.
+    inv INIT. rr. ss.
+    split; eauto.
+    des_ifs. ss.
+    ii.
+    generalize sound_genv; intro SG.
+    exploit SG; ss; eauto.
+    intro T. des. des_ifs.
+    clear SG.
+    exploit NTHIDX; eauto. intro T; des. clarify.
+    unfold load_owned_heaps. des_ifs; cycle 1.
+    {
+      exfalso. folder.
+      clear - NTH Heq.
+      exploit nth_error_Some. rewrite NTH. intro Q. ss.
+      desH Q. clear Q0. exploit Q; eauto. { ss. } intro QQ.
+      erewrite nth_error_None in *; eauto. ss. xomega.
+    }
+    unfold upcast. ss.
+    f_equal.
+    clarify.
+  Qed.
+
+  Theorem sound_progress
+          st0 tr st1
+          (SS: sound_state st0)
+          (STEP: Step sem st0 tr st1)
+    :
+      <<SS: sound_state st1>>
+  .
+  Proof.
+    generalize (sound_genv p); intro SG.
+    inv STEP; ss.
+    - (* call *)
+      rr in SS; des. rr; ss; des_ifs.
+      split; eauto. ii.
+      unfold Midx.update. des_ifs.
+      + exploit SG; ss; eauto. intro T. des. ss.
+        exploit nth_error_In; eauto. intro IN.
+        r. f_equal. eapply UNIQ; eauto.
+        { rewrite Forall_forall in *.
+          eapply FRAMES; ss; eauto. }
+        exploit NTHIDX; eauto.
+      + eapply WTY; eauto.
+    - (* init *)
+      rr in SS; des. rr; ss; des_ifs.
+      esplits; eauto.
+      econs; ss; eauto.
+      inv MSFIND. ss.
+    - (* internal *)
+      rr in SS; des. rr; ss; des_ifs.
+      esplits; eauto.
+      inv FRAMES.
+      econs; ss; eauto.
+    - (* return *)
+      rr in SS; des. rr; ss; des_ifs.
+      esplits; eauto; cycle 1.
+      { inv FRAMES. inv H2. econs; eauto. }
+      ii.
+      unfold Midx.update. des_ifs.
+      + exploit SG; ss; eauto. intro T. des. ss.
+        exploit nth_error_In; eauto. intro IN.
+        f_equal. eapply UNIQ; eauto.
+        { rewrite Forall_forall in *.
+          eapply FRAMES; ss; eauto. }
+        exploit NTHIDX; eauto.
+      + eapply WTY; eauto.
+  Qed.
+
+End PRSV.
+End SemPrsv.
