proof/SemProps.v
@@ -15,8 +15,13 @@ Require Import SimSymb SimMem.
 
 Require Import ModSemProps.
 Require Import Program.
+Require Import Any.
 
 Set Implicit Arguments.
+
+
+
+
 
 
 (* TODO: better namespace? *)
@@ -527,7 +532,7 @@ Proof.
       { econs; et. }
       i. determ_tac ModSem.final_frame_dtm.
       repeat f_equal. eapply ModSem.after_external_dtm; et.
-      rp; eauto. rewrite OH in *. simpl_depind. clarify.
+      rp; eauto. rewrite OH in *. clarify. simpl_depind. clarify.
   - ss. inv FINAL. ss. inv STEP; ss; ModSem.tac.
   - inv H; s; try omega. exploit sd_traces_at; eauto.
 Qed.
